\begin{proof}
	We prove this by induction on $r \leq s$ when $A_r$ and $B_s$ are simple $r$- and $s$-vectors respectively.

	The case $r=1,\quad s=1$ is true by Definition \ref{t:geometric-product}.
	The case $r=1,\quad s>1$ is true by Lemma \ref{l:v-mv-product}.
	Assume the expression holds for $r = q,\quad s > r$, we show that it holds for $r+1$:
	\begin{align*}
		A_{r+1}B_s = &a_{r+1}A_rB_s = a_{r+1}\sum_{k=0}^r \g{A_rB_s}{s-r+2k} = \\
		= &\sum_{k=0}^r a_{r+1}\g{A_rB_s}{s-r+2k} = \\
		= &\sum_{k=0}^r \left[a_{r+1} | \g{A_rB_s}{s-r+2k} + a_{r+1} \wedge \g{A_rB_s}{s-r+2k}\right]\\
		= &a | \g{A_rB_s}{s-r} \\
		  + &\sum_{k=1}^r \left[a_{r+1} | \g{A_rB_s}{s-r+2k} + a_{r+1} \wedge \g{A_rB_s}{s-r+2(k-1)}\right]\\
		  + &a\wedge \g{A_rB_s}{s+r}
	\end{align*}
	where in the last step, we have grouped terms together by grade:
	\begin{align*}
		&\g{A_{r+1}B_s}{s-(r+1)} \equiv a_{r+1} | \g{A_rB_s}{s-r} \\
		&\g{A_{r+1}B_s}{s-(r+1)+2k} \equiv a | \g{A_rB_s}{s-r+2k} + a \wedge \g{A_rB_s}{s-r+2(k-1)} \\
		&\g{A_{r+1}B_s}{r+1+s} \equiv a \wedge \g{A_rB_s}{s+r}
	\end{align*}

	The case where $s \leq r$ follows by induction on $s$ (the same argument as above).
	The general case for homogeneous multivectors follows by distributivity of the geometric product.
\end{proof}
